First batch of changes for TLS codec panic freedom proofs.

engine/lib/phases/phase_functionalize_loops.ml
@@ -314,7 +314,7 @@ struct
           in
           let variant = UB.make_closure [ bpat ] variant variant.span in
           UB.call fold_operator
-            [ condition; invariant; variant; init; body ]
+            [ invariant; condition; variant; init; body ]
             span (dty span expr.typ)
       | Loop _ ->
           Error.unimplemented ~issue_id:933 ~details:"Unhandled loop kind" span
